SeparationLogic/Semantics/Up2Flat.v
@@ -1,0 +1,134 @@
+Require Import Coq.Logic.Classical_Prop.
+Require Import Coq.Classes.RelationClasses.
+Require Import Coq.Relations.Relation_Definitions.
+Require Import Logic.lib.Coqlib.
+Require Import Logic.lib.Ensembles_ext.
+Require Import Logic.GeneralLogic.Base.
+Require Import Logic.MinimunLogic.Syntax.
+Require Import Logic.PropositionalLogic.Syntax.
+Require Import Logic.SeparationLogic.Syntax.
+Require Import Logic.PropositionalLogic.KripkeModel.
+Require Import Logic.SeparationLogic.Model.SeparationAlgebra.
+Require Import Logic.SeparationLogic.Model.OrderedSA.
+Require Import Logic.SeparationLogic.Model.DownwardsClosure.
+Require Import Logic.PropositionalLogic.Semantics.Kripke.
+Require Logic.SeparationLogic.Semantics.UpwardsSemantics.
+Require Logic.SeparationLogic.Semantics.FlatSemantics.
+
+Local Open Scope logic_base.
+Local Open Scope syntax.
+Local Open Scope kripke_model.
+Import PropositionalLanguageNotation.
+Import SeparationLogicNotation.
+Import KripkeModelFamilyNotation.
+
+Module Up2Flat.
+Section Up2Flat.
+
+Context {L: Language}
+        {nL: NormalLanguage L}
+        {pL: PropositionalLanguage L}
+        {sL: SeparationLanguage L}
+        {MD: Model}
+        {kMD: KripkeModel MD}
+        {M: Kmodel}
+        {R: Relation (Kworlds M)}
+        {kiM: KripkeIntuitionisticModel (Kworlds M)}
+        {J: Join  (Kworlds M)}
+        {SA: SeparationAlgebra (Kworlds M)}
+        {uSA: UpwardsClosedSeparationAlgebra (Kworlds M)}
+        {SM: Semantics L MD}
+        {kiSM: KripkeIntuitionisticSemantics L MD M SM}
+        {usSM: UpwardsSemantics.SeparatingSemantics L MD M SM}.
+
+Definition fsSM: @FlatSemantics.SeparatingSemantics L sL MD kMD M _ (DownwardsClosure_J) SM.
+Proof.
+  constructor.
+  + (* sat_sepcon *)
+    intros.
+    unfold WeakSemantics.sepcon.
+    split; unfold Included, Ensembles.In; intros m ?.
+    - rewrite (app_same_set (UpwardsSemantics.denote_sepcon _ _) m) in H.
+      destruct H as [m1 [m2 [? [? ?]]]].
+      exists m1, m2.
+      split; [| split]; auto.
+      exists m1, m2.
+      split; [| split]; auto; reflexivity.
+    - rewrite (app_same_set (UpwardsSemantics.denote_sepcon _ _) m).
+      destruct H as [m1 [m2 [[n1 [n2 [? [? ?]]]] [? ?]]]].
+      exists n1, n2.
+      split; [| split]; auto; eapply sat_mono; eauto.
+  + (* sat_wand *)
+    intros.
+    unfold WeakSemantics.wand.
+    split; unfold Included, Ensembles.In; intros m ?.
+    - rewrite (app_same_set (UpwardsSemantics.denote_wand _ _) m) in H.
+      intros.
+      destruct H0 as [m' [m1' [? [? ?]]]].
+      apply (H  _ _ _ H0 H3).
+      eapply sat_mono; eauto.
+    - rewrite (app_same_set (UpwardsSemantics.denote_wand _ _) m).
+      hnf; intros.
+      apply (H m1 m2); auto.
+      exists m0, m1.
+      split; [| split]; auto.
+      reflexivity.
+Qed.
+
+Definition feSM {s'L: SeparationEmpLanguage L} {USA': UnitalSeparationAlgebra' (Kworlds M)} {ueSM: UpwardsSemantics.EmpSemantics L MD M SM}: @FlatSemantics.EmpSemantics L _ _ MD _ M _ (DownwardsClosure_J) SM.
+Proof.
+  constructor;
+  intros m; simpl; unfold Ensembles.In; unfold WeakSemantics.emp;
+  rewrite <- DownwardsClosure_increasing;
+  apply UpwardsSemantics.denote_emp.
+Qed.
+
+End Up2Flat.
+End Up2Flat.
+
+(*
+Module Upwards2Downwards.
+
+Definition usSM {L: Language} {nL: NormalLanguage L} {pL: PropositionalLanguage L} {SL: SeparationLanguage L} {MD: Model} {kMD: KripkeModel MD} (M: Kmodel) {kiM: KripkeIntuitionisticModel (Kworlds M)} {J: Join (Kworlds M)} {SA: SeparationAlgebra (Kworlds M)} {dSA: UpwardsClosedSeparationAlgebra (Kworlds M)} (SM: Semantics L MD) {kiSM: KripkeIntuitionisticSemantics L MD M SM} {usSM: UpwardsSemantics L MD M SM}: @DownwardsSemantics.DownwardsSemantics L nL pL SL MD kMD M kiM (DownwardsClosure_J) SM kiSM.
+Proof.
+  constructor.
+  + (* sat_sepcon *)
+    intros.
+    pose proof Korder_PreOrder as H_PreOrder.
+    rewrite UpwardsSemantics.sat_sepcon.
+    split; intros.
+    - destruct H as [m1 [m2 [? [? ?]]]].
+      exists m, m1, m2.
+      split; [reflexivity |].
+      split; [| split]; auto.
+      exists m1, m2.
+      split; [| split]; auto; reflexivity.
+    - destruct H as [m0 [m1 [m2 [? [[n1 [n2 [? [? ?]]]] [? ?]]]]]].
+      destruct (join_Korder_up m0 m _ _ H2 H) as [n1' [n2' [? [? ?]]]].
+      exists n1', n2'.
+      split; [| split]; auto; eapply sat_mono; eauto; eapply sat_mono; eauto.
+  + (* sat_wand *)
+    intros.
+    pose proof Korder_PreOrder as H_PreOrder.
+    rewrite UpwardsSemantics.sat_wand.
+    split; intros.
+    - destruct H0 as [m' [m1' [? [? ?]]]].
+      apply (H  _ _ _ H0 H3).
+      eapply sat_mono; eauto.
+    - apply (H m1 m2); auto.
+      exists m0, m1.
+      split; [| split]; auto.
+      reflexivity.
+Defined.
+
+(*
+Definition UsSM {L: Language} {nL: NormalLanguage L} {pL: PropositionalLanguage L} {SL: SeparationLanguage L} {uSL: UnitarySeparationLanguage L} {MD: Model} {kMD: KripkeModel MD} (M: Kmodel) {kiM: KripkeIntuitionisticModel (Kworlds M)} {J: Join (Kworlds M)} {SA: SeparationAlgebra (Kworlds M)} {dSA: UpwardsClosedSeparationAlgebra (Kworlds M)} {USA: UnitalSeparationAlgebra (Kworlds M)} {SM: Semantics L MD} {kiSM: KripkeIntuitionisticSemantics L MD M SM} {dsSM: UpwardsSemantics L MD M SM} {UsSM: UnitalSemantics L MD M SM} : @UnitalSemantics L _ _ _ _ MD _ M kiM (DownwardsClosure_SA) SM kiSM.
+Proof.
+  intros m; simpl.
+  rewrite <- DownwardsClosure_nonpositive.
+  apply sat_emp.
+Qed.
+*)
+
+End Upwards2Downwards.
+*)
